src/3d/prelude/EverParse3d.CopyBuffer.fsti
@@ -1,0 +1,6 @@
+module EverParse3d.CopyBuffer
+module I = EverParse3d.InputStream.All
+
+val t : Type0
+
+val as_input_stream : t -> (sl:I.t & I.tlen sl)
